Add lemmas for memory helpers

CHERI_Instantiation.thy
@@ -64,6 +64,7 @@ qed
 section \<open>Simplification rules\<close>
 
 declare zero_extend_def[simp]
+declare CAPABILITY_DBYTES_def[simp]
 
 lemma Bit_bitU_of_bool[simp]: "Morello.Bit w = bitU_of_bool (w !! 0)"
   by (auto simp: Morello.Bit_def)
@@ -80,6 +81,47 @@ lemma CapIsTagSet_CapSetTag_iff[simp]:
   "CapIsTagSet (CapSetTag c t) \<longleftrightarrow> (t !! 0)"
   by (auto simp: test_bit_set)
 
+lemma no_Run_EndOfInstruction[simp]:
+  "Run (EndOfInstruction u) t a \<longleftrightarrow> False"
+  by (auto simp: EndOfInstruction_def)
+
+lemma no_Run_AArch64_TakeException[simp]:
+  "Run (AArch64_TakeException target_el exception preferred_exception_return vect_offset) t a \<longleftrightarrow> False"
+  unfolding AArch64_TakeException_def bind_assoc
+  by (auto elim!: Run_bindE)
+
+lemma no_Run_AArch64_DataAbort[simp]:
+  "Run (AArch64_DataAbort vaddress fault) t a \<longleftrightarrow> False"
+  by (auto simp: AArch64_DataAbort_def elim!: Run_bindE Run_ifE)
+
+lemma no_Run_AArch64_InstructionAbort[simp]:
+  "Run (AArch64_InstructionAbort vaddress fault) t a \<longleftrightarrow> False"
+  by (auto simp: AArch64_InstructionAbort_def elim!: Run_bindE Run_ifE)
+
+lemma no_Run_AArch64_WatchpointException[simp]:
+  "Run (AArch64_WatchpointException vaddress fault) t a \<longleftrightarrow> False"
+  by (auto simp: AArch64_WatchpointException_def elim!: Run_bindE Run_ifE)
+
+lemma no_Run_AArch64_BreakpointException[simp]:
+  "Run (AArch64_BreakpointException fault) t a \<longleftrightarrow> False"
+  by (auto simp: AArch64_BreakpointException_def elim!: Run_bindE Run_ifE)
+
+lemma no_Run_AArch64_Abort[simp]:
+  "Run (AArch64_Abort vaddress fault) t a \<longleftrightarrow> False"
+  by (auto simp: AArch64_Abort_def elim!: Run_bindE Run_ifE)
+
+lemma if_no_Run_then_else:
+  assumes "\<not>Run m1 t a"
+  shows "Run (if c then m1 else m2) t a \<longleftrightarrow> \<not>c \<and> Run m2 t a"
+  using assms
+  by auto
+
+lemma unat_paddress_plus_16[simp]:
+  "unat (ucast (FullAddress_address (AddressDescriptor_paddress desc)) + (16 :: 64 word))
+   = unat (FullAddress_address (AddressDescriptor_paddress desc)) + 16"
+  sorry
+
+
 lemmas datatype_splits =
   ArchVersion.splits Constraint.splits Unpredictable.splits Exception.splits InstrEnc.splits
   BranchType.splits Fault.splits AccType.splits DeviceType.splits MemType.splits InstrSet.splits
@@ -88,8 +130,7 @@ lemmas datatype_splits =
   CountOp.splits ExtendType.splits FPMaxMinOp.splits FPUnaryOp.splits FPConvOp.splits
   MoveWideOp.splits ShiftType.splits LogicalOp.splits MemOp.splits MemAtomicOp.splits
   MemBarrierOp.splits SystemHintOp.splits PSTATEField.splits SystemOp.splits VBitOp.splits
-  CompareOp.splits ImmediateOp.splits ReduceOp.splits SRType.splits AsyncErrorType.splits
-  VBitOps.splits VCGEtype.splits VCGTtype.splits VFPNegMul.splits
+  CompareOp.splits ImmediateOp.splits ReduceOp.splits AsyncErrorType.splits
 
 section \<open>Capabilities\<close>
 
@@ -227,7 +268,7 @@ definition "ISA \<equiv>
    tag_granule = 16,
    PCC = {''PCC''},
    KCC = {''CVBAR_EL1'', ''CVBAR_EL2'', ''CVBAR_EL3''},
-   IDC = {''R29''},
+   IDC = {''_R29''},
    isa.caps_of_regval = caps_of_regval,
    isa.invokes_caps = invokes_caps,
    isa.instr_raises_ex = instr_raises_ex,
@@ -242,11 +283,12 @@ sublocale Capability_ISA CC ISA ..
 lemma ISA_simps[simp]:
   "PCC ISA = {''PCC''}"
   "KCC ISA = {''CVBAR_EL1'', ''CVBAR_EL2'', ''CVBAR_EL3''}"
-  "IDC ISA = {''R29''}"
+  "IDC ISA = {''_R29''}"
   "privileged_regs ISA = {''CVBAR_EL1'', ''CVBAR_EL2'', ''CVBAR_EL3''}"
   "isa.instr_sem ISA = instr_sem"
   "isa.instr_fetch ISA = instr_fetch"
   "isa.caps_of_regval ISA = caps_of_regval"
+  "isa.is_translation_event ISA = is_translation_event"
   by (auto simp: ISA_def)
 
 lemma no_cap_regvals[simp]:
@@ -260,11 +302,10 @@ lemma no_cap_regvals[simp]:
   "\<And>v. bitvector_128_dec_of_regval rv = Some v \<Longrightarrow> caps_of_regval rv = {}"
   "\<And>v. bitvector_16_dec_of_regval rv = Some v \<Longrightarrow> caps_of_regval rv = {}"
   "\<And>v. bitvector_1_dec_of_regval rv = Some v \<Longrightarrow> caps_of_regval rv = {}"
-  "\<And>v. bitvector_29_dec_of_regval rv = Some v \<Longrightarrow> caps_of_regval rv = {}"
   "\<And>v. bitvector_2_dec_of_regval rv = Some v \<Longrightarrow> caps_of_regval rv = {}"
   "\<And>v. bitvector_32_dec_of_regval rv = Some v \<Longrightarrow> caps_of_regval rv = {}"
   "\<And>v. bitvector_4_dec_of_regval rv = Some v \<Longrightarrow> caps_of_regval rv = {}"
-  "\<And>v. bitvector_52_dec_of_regval rv = Some v \<Longrightarrow> caps_of_regval rv = {}"
+  "\<And>v. bitvector_48_dec_of_regval rv = Some v \<Longrightarrow> caps_of_regval rv = {}"
   "\<And>v. bitvector_63_dec_of_regval rv = Some v \<Longrightarrow> caps_of_regval rv = {}"
   "\<And>v. bitvector_64_dec_of_regval rv = Some v \<Longrightarrow> caps_of_regval rv = {}"
   "\<And>v. bool_of_regval rv = Some v \<Longrightarrow> caps_of_regval rv = {}"
@@ -282,39 +323,24 @@ locale Morello_Fixed_Address_Translation =
   fixes translate_address :: "nat \<Rightarrow> acctype \<Rightarrow> nat option"
     and is_translation_event :: "register_value event \<Rightarrow> bool"
     and translation_assms :: "register_value event \<Rightarrow> bool"
-  assumes translate_correct64:
+  assumes translate_correct:
       "\<And>vaddress acctype iswrite wasaligned size iswritevalidcap addrdesc.
           Run (AArch64_TranslateAddressWithTag vaddress acctype iswrite wasaligned size iswritevalidcap) t addrdesc \<Longrightarrow>
           FaultRecord_statuscode (AddressDescriptor_fault addrdesc) = Fault_None \<Longrightarrow>
           \<forall>e \<in> set t. translation_assms e \<Longrightarrow>
           translate_address (unat vaddress) (acctype_of_AccType acctype iswrite) =
             Some (unat (FullAddress_address (AddressDescriptor_paddress addrdesc)))"
-    and translate_correct32:
-      "\<And>vaddress acctype iswrite wasaligned size iswritevalidcap addrdesc.
-          Run (AArch32_TranslateAddressWithTag vaddress acctype iswrite wasaligned size iswritevalidcap) t addrdesc \<Longrightarrow>
-          FaultRecord_statuscode (AddressDescriptor_fault addrdesc) = Fault_None \<Longrightarrow>
-          \<forall>e \<in> set t. translation_assms e \<Longrightarrow>
-          translate_address (unat vaddress) (acctype_of_AccType acctype iswrite) =
-            Some (unat (FullAddress_address (AddressDescriptor_paddress addrdesc)))"
-    and is_translation_event_correct64:
+    and is_translation_event_correct:
       "\<And>vaddress acctype iswrite wasaligned size iswritevalidcap addrdesc e.
           Run (AArch64_TranslateAddressWithTag vaddress acctype iswrite wasaligned size iswritevalidcap) t addrdesc \<Longrightarrow>
-          \<forall>e' \<in> set t. translation_assms e' \<Longrightarrow>
-          e \<in> set t \<Longrightarrow> is_mem_event e \<Longrightarrow>
-          is_translation_event e"
-    and is_translation_event_correct32:
-      "\<And>vaddress acctype iswrite wasaligned size iswritevalidcap addrdesc e.
-          Run (AArch32_TranslateAddressWithTag vaddress acctype iswrite wasaligned size iswritevalidcap) t addrdesc \<Longrightarrow>
           \<forall>e' \<in> set t. translation_assms e' \<Longrightarrow>
           e \<in> set t \<Longrightarrow> is_mem_event e \<Longrightarrow>
           is_translation_event e"
 begin
 
-(* sublocale Capability_ISA CC ISA .. *)
-
 sublocale Morello_ISA where translate_address = "\<lambda>addr acctype _. translate_address addr acctype" .
 
-sublocale Capability_ISA_Fixed_Translation CC ISA "\<lambda>t. \<forall>e \<in> set t. translation_assms e"
+sublocale Capability_ISA_Fixed_Translation CC ISA translation_assms
   by unfold_locales (auto simp: ISA_def)
 
 end
@@ -322,21 +348,20 @@ end
 text \<open>Instantiation of translate_address for version of spec with translation stubs\<close>
 
 definition translate_address :: "nat \<Rightarrow> acctype \<Rightarrow> nat option" where
-  "translate_address addr acctype \<equiv> Some (addr mod 2^52)"
+  "translate_address addr acctype \<equiv> Some (addr mod 2^48)"
 
 lemmas TranslateAddress_defs =
   AArch64_TranslateAddress_def AArch64_TranslateAddressWithTag_def AArch64_FullTranslateWithTag_def
   AArch64_FirstStageTranslateWithTag_def AArch64_SecondStageTranslate_def
-  AArch32_TranslateAddressWithTag_def AArch32_FullTranslateWithTag_def
-  AArch32_FirstStageTranslateWithTag_def AArch32_SecondStageTranslate_def
   translate_address_def
 
-lemma unat64_and_mask52_mod: "unat ((w :: 64 word) AND mask 52) = unat w mod 2^52"
+(*lemma unat64_and_mask52_mod: "unat ((w :: 64 word) AND mask 52) = unat w mod 2^52"
   by (auto simp: and_mask_bintr unat_def uint_word_of_int bintrunc_mod2p nat_mod_distrib)
 
 lemma unat32_and_mask52_eq: "unat (w :: 32 word) mod 4503599627370496 = unat w"
   using unat_lt2p[of w]
-  by auto
+  by auto*)
+
 
 interpretation Morello_Fixed_Address_Translation
   where translate_address = translate_address
@@ -404,9 +429,9 @@ declare datatype_splits[where P = "non_mem_exp", non_mem_exp_split]
 
 end
 
-locale Morello_Axiom_Assm_Automaton = Morello_Axiom_Automaton +
+(*locale Morello_Axiom_Assm_Automaton = Morello_Axiom_Automaton +
   fixes ex_traces :: bool
-    and ev_assm :: "register_value event \<Rightarrow> bool"
+    and ev_assms :: "register_value event \<Rightarrow> bool"
   assumes non_cap_event_enabled: "\<And>e. non_cap_event e \<Longrightarrow> enabled s e"
     and read_non_special_regs_enabled: "\<And>r v. r \<notin> PCC ISA \<union> IDC ISA \<union> KCC ISA \<union> privileged_regs ISA \<Longrightarrow> enabled s (E_read_reg r v)"
 begin
@@ -414,7 +439,7 @@ begin
 sublocale Cap_Axiom_Assm_Automaton where CC = CC and ISA = ISA
   by unfold_locales (blast intro: non_cap_event_enabled read_non_special_regs_enabled)+
 
-end
+end*)
 
 locale Morello_Write_Cap_Automaton = Morello_ISA +
   fixes ex_traces :: bool and invoked_caps :: "Capability set"
@@ -425,18 +450,306 @@ fun ev_assms :: "register_value event \<Rightarrow> bool" where
   "ev_assms (E_read_reg r v) = (r = ''PCC'' \<longrightarrow> (\<forall>c \<in> caps_of_regval v. \<not>CapIsSealed c))"
 | "ev_assms _ = True"
 
-sublocale Write_Cap_Assm_Automaton where CC = CC and ISA = ISA ..
+sublocale Write_Cap_Assm_Automaton where CC = CC and ISA = ISA and ev_assms = ev_assms ..
+
+sublocale Morello_Axiom_Automaton where enabled = enabled ..
 
 end
 
-locale Morello_Mem_Automaton = Morello_Fixed_Address_Translation +
-  fixes is_fetch :: bool and ex_traces :: bool
+(* Assume stubbed out address translation for now *)
+locale Morello_Mem_Automaton =
+  Morello_Fixed_Address_Translation
+  where translate_address = translate_address
+    and is_translation_event = "\<lambda>_. False"
+    and translation_assms = "\<lambda>_. True" +
+  fixes ex_traces :: bool
 begin
 
-sublocale Mem_Assm_Automaton where CC = CC and ISA = ISA
-  and translation_assms = "\<lambda>t. \<forall>e \<in> set t. translation_assms e"
-  and ev_assms = "\<lambda>e. True" \<comment> \<open>TODO\<close>
+sublocale Mem_Assm_Automaton
+  where CC = CC and ISA = ISA
+    and translation_assms = "\<lambda>_. True"
+    and is_fetch = "False"
+    and extra_assms = "\<lambda>e. True" \<comment> \<open>TODO\<close>
   ..
+
+sublocale Morello_Axiom_Automaton
+  where translate_address = "\<lambda>addr acctype _. translate_address addr acctype"
+    and enabled = enabled
+    and is_translation_event = "\<lambda>_. False"
+  ..
+
+term ReadMemory
+term access_enabled
+
+lemma nat_of_bv_mword_unat[simp]: "nat_of_bv BC_mword w = Some (unat w)"
+  by (auto simp: nat_of_bv_def unat_def)
+
+lemma access_enabled_runI[derivable_caps_runI]:
+  assumes "access_enabled s acctype addr sz v tag"
+  shows "access_enabled (run s t) acctype addr sz v tag"
+  using assms derivable_mono[OF accessed_caps_run_mono]
+  by (auto simp: access_enabled_def)
+
+lemma traces_enabled_ReadMemory:
+  assumes "\<And>v. access_enabled s Load (unat paddr) sz v B0"
+  shows "traces_enabled (ReadMemory sz paddr) s"
+  using assms
+  unfolding ReadMemory_def
+  by (intro traces_enabled_read_mem) (auto)
+
+lemma traces_enabled_Mem_read[traces_enabledI]:
+  assumes "\<And>v. access_enabled s Load (unat (FullAddress_address (AddressDescriptor_paddress desc))) (nat sz) v B0"
+  shows "traces_enabled (Mem_read desc sz accdesc) s"
+  unfolding Mem_read_def bind_assoc
+  by (traces_enabledI intro: traces_enabled_read_mem assms: assms)
+
+lemma traces_enabled_ReadMem[traces_enabledI]:
+  assumes "\<And>v. access_enabled s Load (unat (FullAddress_address (AddressDescriptor_paddress desc))) (nat sz) v B0"
+  shows "traces_enabled (ReadMem desc sz accdesc) s"
+  unfolding ReadMem_def bind_assoc
+  by (traces_enabledI intro: traces_enabled_read_mem assms: assms)
+
+lemma traces_enabled_ReadTaggedMem[traces_enabledI]:
+  assumes "\<And>v tag. access_enabled s Load (unat (FullAddress_address (AddressDescriptor_paddress desc))) 16 v tag"
+    and "\<And>v tag. sz = 32 \<Longrightarrow> access_enabled s Load (unat (FullAddress_address (AddressDescriptor_paddress desc)) + 16) 16 v tag"
+    and "sz = 16 \<or> sz = 32"
+  shows "traces_enabled (ReadTaggedMem desc sz accdesc) s"
+  unfolding ReadTaggedMem_def bind_assoc
+  by (traces_enabledI intro: traces_enabled_read_memt non_cap_expI[THEN non_cap_exp_traces_enabledI] access_enabled_runI assms: assms)
+
+lemma traces_enabled_ReadTags[traces_enabledI]:
+  assumes "\<And>i v tag. i < nat sz \<Longrightarrow> access_enabled s Load (unat (FullAddress_address (AddressDescriptor_paddress desc)) + (i * 16)) 16 v tag"
+  shows "traces_enabled (ReadTags desc sz accdesc) s"
+  unfolding ReadTags_def bind_assoc
+  by (traces_enabledI intro: traces_enabled_read_memt non_cap_expI[THEN non_cap_exp_traces_enabledI] access_enabled_runI
+                      assms: assms)
+
+lemma traces_enabled_Write_mem:
+  assumes "\<And>r. traces_enabled (m r) (axiom_step s (E_write_mem wk paddr sz v r))"
+    and "\<And>r. enabled s (E_write_mem wk paddr sz v r)"
+  shows "traces_enabled (Write_mem wk paddr sz v m) s"
+  using assms
+  by (fastforce simp: traces_enabled_def elim!: Traces_cases[where m = "Write_mem wk paddr sz v m"])
+
+lemma length_take_chunks:
+  assumes "n > 0" and "n dvd length xs"
+  shows "length (take_chunks n xs) = length xs div n"
+proof (use assms in \<open>induction n xs rule: take_chunks.induct[case_names Nil Zero Take]\<close>)
+  case (Take n xs)
+  then show ?case
+    by (cases "length xs < n") (auto simp: div_geq)
+qed auto
+
+lemma length_mem_bytes_of_word:
+  fixes w :: "'a::len word"
+  assumes "8 dvd LENGTH('a)"
+  shows "length (mem_bytes_of_word w) = LENGTH('a) div 8"
+  using assms
+  by (auto simp add: mem_bytes_of_word_def length_take_chunks simp del: take_chunks.simps)
+
+lemma traces_enabled_write_mem:
+  fixes data :: "'a::len word"
+  assumes "access_enabled s Store (unat paddr) (nat sz) (mem_bytes_of_word data) B0"
+    and "LENGTH('a) = nat sz * 8" and "sz > 0"
+  shows "traces_enabled (write_mem BC_mword BC_mword wk addr_sz paddr sz data) s"
+  using assms
+  unfolding write_mem_def
+  by (auto intro!: traces_enabled_Write_mem non_cap_expI[THEN non_cap_exp_traces_enabledI]
+           split: option.splits simp: legal_store_def length_mem_bytes_of_word)
+
+lemma traces_enabled_Mem_set[traces_enabledI]:
+  fixes data :: "'a::len word"
+  assumes "access_enabled s Store (unat (FullAddress_address (AddressDescriptor_paddress desc))) (nat sz) (mem_bytes_of_word data) B0"
+    and "LENGTH('a) = nat sz * 8" and "sz > 0"
+  shows "traces_enabled (Mem_set desc sz accdesc data) s"
+  using assms
+  unfolding Mem_set_def
+  by (auto intro!: traces_enabled_bind traces_enabled_write_mem non_cap_expI[THEN non_cap_exp_traces_enabledI])
+
+lemma traces_enabled_Write_memt:
+  assumes "\<And>r. traces_enabled (m r) (axiom_step s (E_write_memt wk paddr sz v tag r))"
+    and "\<And>r. enabled s (E_write_memt wk paddr sz v tag r)"
+  shows "traces_enabled (Write_memt wk paddr sz v tag m) s"
+  using assms
+  by (fastforce simp: traces_enabled_def elim!: Traces_cases[where m = "Write_memt wk paddr sz v tag m"])
+
+fun bitU_nonzero :: "bitU \<Rightarrow> bool" where
+  "bitU_nonzero B0 = False"
+| "bitU_nonzero _ = True"
+
+definition Capability_of_tag_word :: "bool \<Rightarrow> 128 word \<Rightarrow> Capability" where
+  "Capability_of_tag_word tag word =
+     (let tag = (of_bl [tag] :: 1 word) in
+      word_cat tag word)"
+
+lemma traces_enabled_write_memt:
+  fixes data :: "128 word"
+  assumes "access_enabled s Store (unat paddr) 16 (mem_bytes_of_word data) tag"
+    and "tag = B0 \<or> tag = B1"
+    and "tag \<noteq> B0 \<Longrightarrow> Capability_of_tag_word (bitU_nonzero tag) data \<in> derivable_caps s"
+  shows "traces_enabled (write_memt BC_mword BC_mword wk paddr 16 data tag) s"
+  using assms
+  unfolding write_memt_def
+  by (auto intro!: traces_enabled_Write_memt non_cap_expI[THEN non_cap_exp_traces_enabledI]
+           split: option.splits simp: legal_store_def length_mem_bytes_of_word)
+
+lemma traces_enabled_WriteTaggedMem_single[traces_enabledI]:
+  fixes tag :: "1 word" and data :: "128 word"
+  assumes "access_enabled s Store (unat (FullAddress_address (AddressDescriptor_paddress desc))) 16 (mem_bytes_of_word data) (bitU_of_bool (tag !! 0))"
+    and "Capability_of_tag_word (tag !! 0) data \<in> derivable_caps s"
+  shows "traces_enabled (WriteTaggedMem desc 16 accdesc tag data) s"
+  using assms
+  unfolding WriteTaggedMem_def
+  by (cases "tag !! 0")
+     (auto intro!: traces_enabled_write_memt traces_enabled_bind non_cap_expI[THEN non_cap_exp_traces_enabledI])
+
+lemma run_write_memt:
+  assumes "Run (write_memt BC_a BC_b wk paddr sz v tag) t a"
+  shows "run s t = s"
+  using assms
+  by (auto simp add: write_memt_def split: option.splits elim!: Write_memt_TracesE)
+
+lemma traces_enabled_WriteTaggedMem_pair[traces_enabledI]:
+  fixes tags :: "2 word" and data :: "256 word"
+  assumes "access_enabled s Store (unat (FullAddress_address (AddressDescriptor_paddress desc))) 16 (mem_bytes_of_word (ucast data :: 128 word)) (bitU_of_bool (tags !! 0))"
+    and "access_enabled s Store (unat (FullAddress_address (AddressDescriptor_paddress desc)) + 16) 16 (mem_bytes_of_word (Word.slice 128 data :: 128 word)) (bitU_of_bool (tags !! 1))"
+    and "Capability_of_tag_word (tags !! 0) (ucast data) \<in> derivable_caps s"
+    and "Capability_of_tag_word (tags !! 1) (Word.slice 128 data) \<in> derivable_caps s"
+  shows "traces_enabled (WriteTaggedMem desc 32 accdesc tags data) s"
+  using assms
+  unfolding WriteTaggedMem_def
+  by (cases "tags !! 0"; cases "tags !! 1")
+     (auto intro!: traces_enabled_write_memt traces_enabled_bind non_cap_expI[THEN non_cap_exp_traces_enabledI]
+           simp: run_write_memt)
+
+lemma traces_enabled_WriteTaggedMem[traces_enabledI]:
+  fixes tags :: "'t::len word" and data :: "'d::len word"
+  assumes "access_enabled s Store (unat (FullAddress_address (AddressDescriptor_paddress desc))) 16 (mem_bytes_of_word (ucast data :: 128 word)) (bitU_of_bool (tags !! 0))"
+    and "Capability_of_tag_word (tags !! 0) (ucast data) \<in> derivable_caps s"
+    and "sz = 32 \<Longrightarrow> access_enabled s Store (unat (FullAddress_address (AddressDescriptor_paddress desc)) + 16) 16 (mem_bytes_of_word (Word.slice 128 data :: 128 word)) (bitU_of_bool (tags !! 1))"
+    and "sz = 32 \<Longrightarrow> Capability_of_tag_word (tags !! 1) (Word.slice 128 data) \<in> derivable_caps s"
+    and "sz = 16 \<or> sz = 32"
+    and "LENGTH('t) = nat sz div 16" and "LENGTH('d) = 8 * nat sz"
+  shows "traces_enabled (WriteTaggedMem desc sz accdesc tags data) s"
+  using assms
+  unfolding WriteTaggedMem_def
+  by (cases "tags !! 0"; cases "tags !! 1")
+     (auto intro!: traces_enabled_write_memt traces_enabled_bind non_cap_expI[THEN non_cap_exp_traces_enabledI]
+           simp: run_write_memt nth_ucast)
+
+definition store_enabled where
+  "store_enabled s vaddr acctype sz data tag \<equiv>
+     \<forall>paddr.
+        translate_address vaddr (acctype_of_AccType acctype True) = Some paddr \<longrightarrow>
+        access_enabled s Store paddr (nat sz) (mem_bytes_of_word data) (bitU_of_bool tag)"
+
+definition load_enabled where
+  "load_enabled s vaddr acctype sz tagged \<equiv>
+     \<forall>paddr data tag.
+        translate_address vaddr (acctype_of_AccType acctype False) = Some paddr \<longrightarrow>
+        access_enabled s Load paddr (nat sz) data (if tagged then tag else B0)"
+
+lemma store_enabled_runI[derivable_caps_runI]:
+  assumes "store_enabled s vaddr acctype sz data tag"
+  shows "store_enabled (run s t) vaddr acctype sz data tag"
+  using assms
+  by (auto simp: store_enabled_def intro: access_enabled_runI)
+
+lemma load_enabled_runI[derivable_caps_runI]:
+  assumes "load_enabled s vaddr acctype sz tagged"
+  shows "load_enabled (run s t) vaddr acctype sz tagged"
+  using assms
+  by (auto simp: load_enabled_def intro: access_enabled_runI)
+
+(* TODO *)
+lemma
+  assumes "load_enabled s (vaddr + offset) acctype sz tagged"
+    and "translate_address vaddr (acctype_of_AccType acctype False) = Some paddr"
+    and "tagged \<or> tag = B0"
+  shows "access_enabled s Load (paddr + offset) (nat sz) data tag"
+  using assms
+  apply (cases tagged)
+  apply (auto simp: load_enabled_def translate_address_def dvd_def)
+  oops
+
+text \<open>The VirtualAddress type in the ASL\<close>
+
+abbreviation "perm_bits_included perms1 perms2 \<equiv> (perms1 AND perms2) = perms1"
+
+definition VA_derivable :: "VirtualAddress \<Rightarrow> (129 word, register_value) axiom_state \<Rightarrow> bool" where
+  "VA_derivable va s \<equiv>
+     (case VirtualAddress_vatype va of
+        VA_Capability \<Rightarrow> VirtualAddress_base va \<in> derivable_caps s
+      | VA_Bits64 \<Rightarrow> True)"
+
+lemma VA_derivable_run_imp[derivable_caps_runI]:
+  assumes "VA_derivable va s"
+  shows "VA_derivable va (run s t)"
+  using assms
+  by (auto simp: VA_derivable_def split: VirtualAddressType.splits intro: derivable_caps_runI)
+
+lemma BaseReg_read_VA_derivable[derivable_capsE]:
+  assumes "Run (BaseReg_read n is_prefetch) t va"
+    and "{''_R29''} \<subseteq> accessible_regs s"
+  shows "VA_derivable va (run s t)"
+  sorry
+
+declare BaseReg_read_VA_derivable[where is_prefetch = False, folded BaseReg_read__1_def, derivable_capsE]
+
+lemma AltBaseReg_read_VA_derivable[derivable_capsE]:
+  assumes "Run (AltBaseReg_read n is_prefetch) t va"
+    and "{''_R29''} \<subseteq> accessible_regs s"
+  shows "VA_derivable va (run s t)"
+proof (cases "VirtualAddress_vatype va")
+  case VA_Bits64
+  then show ?thesis
+    by (auto simp: VA_derivable_def)
+next
+  case VA_Capability
+  then have "VirtualAddress_base va \<in> derivable_caps (run s t)"
+    using assms
+    unfolding AltBaseReg_read_def
+    apply (auto elim!: Run_bindE Run_ifE)
+    sorry
+  then show ?thesis
+    using VA_Capability
+    by (auto simp: VA_derivable_def)
+qed
+
+declare AltBaseReg_read_VA_derivable[where is_prefetch = False, folded AltBaseReg_read__1_def, derivable_capsE]
+
+lemma VADeref_load_enabled[derivable_capsE]:
+  assumes "Run (VADeref va sz perms acctype) t vaddr"
+    and "perm_bits_included CAP_PERM_LOAD perms"
+    and "tagged \<longrightarrow> perm_bits_included CAP_PERM_LOAD_CAP perms"
+    and "VA_derivable va s"
+    and "{''PCC''} \<subseteq> accessible_regs s"
+  shows "load_enabled (run s t) (unat vaddr) acctype sz tagged"
+  sorry
+
+lemma VADeref_store_data_enabled[derivable_capsE]:
+  assumes "Run (VADeref va sz perms acctype) t vaddr"
+    and "perm_bits_included CAP_PERM_STORE perms"
+    and "VA_derivable va s"
+    and "{''PCC''} \<subseteq> accessible_regs s"
+  shows "store_enabled (run s t) (unat vaddr) acctype sz data False"
+  sorry
+
+lemma VADeref_store_enabled[derivable_capsE]:
+  assumes "Run (VADeref va sz perms acctype) t vaddr"
+    and "perm_bits_included CAP_PERM_STORE perms"
+    and "tag \<longrightarrow> perm_bits_included CAP_PERM_STORE_CAP perms"
+    and "tag \<and> CapIsLocal (Capability_of_tag_word tag data) \<longrightarrow> perm_bits_included CAP_PERM_STORE_LOCAL perms"
+    and "VA_derivable va s"
+    and "{''PCC''} \<subseteq> accessible_regs s"
+  shows "store_enabled (run s t) (unat vaddr) acctype sz data tag"
+  sorry
+
+text \<open>Functions/instructions that need fixing in the ASL\<close>
+
+lemma traces_enabled_DC_ZVA[traces_enabledI]:
+  "traces_enabled (DC_ZVA v) s"
+  sorry
 
 end
 
